More refactoring.

Coherence/DelocationCorrect.v
@@ -1,5 +1,5 @@
-Require Import Util CSet CMap MoreExp SetOperations OUnion.
-Require Import IL InRel RenamedApart LabelsDefined Restrict.
+Require Import Util CSet CMap MapDefined MoreExp SetOperations OUnion.
+Require Import IL InRel4 RenamedApart LabelsDefined Restrict.
 Require Import Annotation Liveness Coherence Delocation.
 Require Import Bisim BisimTactics.
 
@@ -9,76 +9,9 @@ Set Implicit Arguments.
 Unset Printing Records.
 Unset Printing Abstraction Types.
 
-
-Inductive mutual_block {A1 A2 A3 A4} {B} `{BlockType B} {C} `{BlockType C} (R:A1->A2->A3->A4->B->C->Prop)
-: nat -> list A1 -> list A2 -> list A3 -> list A4 -> list B -> list C -> Prop :=
-  | CS_nil n : mutual_block R n nil nil nil nil nil nil
-  | CS_cons a1 a2 a3 a4 b c n AL1 AL2 AL3 AL4 L L' :
-      mutual_block R (S n) AL1 AL2 AL3 AL4 L L'
-      -> n = block_n b
-      -> n = block_n c
-      -> R a1 a2 a3 a4 b c
-      -> mutual_block R n (a1::AL1) (a2::AL2) (a3::AL3) (a4::AL4) (b::L) (c::L').
-
-
-Lemma mutual_block_zero {A1 A2 A3 A4} {B} `{BlockType B} {C} `{BlockType C} (R:A1->A2->A3->A4->B->C->Prop)
-      AL1 AL2 AL3 AL4 (L:list B) (L':list C) n b i
-: mutual_block R i AL1 AL2 AL3 AL4 L L' -> get L n b -> block_n b = (n+i).
-Proof.
-  intros. general induction H2. inv H1; eauto.
-  inv H1; eauto. erewrite IHget; eauto. omega.
-Qed.
-
-Lemma mutual_block_length {A1 A2 A3 A4} {B} `{BlockType B} {C} `{BlockType C} (R:A1->A2->A3->A4->B->C->Prop)
-      AL1 AL2 AL3 AL4 (L1:list B) (L2:list C) i
-: mutual_block R i AL1 AL2 AL3 AL4 L1 L2 -> ❬AL1❭ = ❬L1❭ /\ ❬AL2❭ = ❬L1❭ /\ ❬AL3❭ = ❬L1❭  /\ ❬AL4❭ = ❬L1❭ /\ ❬L2❭ = ❬L1❭.
-Proof.
-  intros. general induction H1; dcr; simpl; eauto.
-  repeat split; omega.
-Qed.
-
-
-Lemma mutual_approx {A1 A2 A3 A4} {B} `{BlockType B} {C} `{BlockType C}
-      (R:list A1 -> list A2 -> list A3 -> list A4 -> list B -> list C ->
-         A1 -> A2 -> A3 -> A4 -> B -> C -> Prop)
-      AL1 AL2 AL3 AL4 AL1' AL2' AL3' AL4' F1 F2 L1 L2
-  : length AL1' = length F1
-    -> length AL1' = length AL2'
-    -> length AL2' = length AL3'
-    -> length AL3' = length AL4'
-    -> length F1 = length F2
-    -> (forall n a1 a2 a3 a4 b b', get AL1' n a1 -> get AL2' n a2 -> get AL3' n a3 -> get AL4' n a4
-                             -> get F1 n b -> get F2 n b' -> R AL1 AL2 AL3 AL4 L1 L2 a1 a2 a3 a4 b b')
-    -> (forall i b, get F1 i b -> i = block_n b)
-    -> (forall i b, get F2 i b -> i = block_n b)
-    -> mutual_block (R AL1 AL2 AL3 AL4 L1 L2) 0 AL1' AL2' AL3' AL4' F1 F2.
-Proof.
-Admitted.
-
-Inductive inRel {A1 A2 A3 A4} {B} `{BlockType B} {C} `{BlockType C}
-          (R:list A1 -> list A2 -> list A3 -> list A4 -> list B -> list C ->
-             A1 -> A2 -> A3 -> A4 -> B -> C -> Prop)
-: list A1 -> list A2 -> list A3 -> list A4 -> list B -> list C -> Prop :=
-  | LPM_nil : inRel R nil nil nil nil nil nil
-  | LPM_app AL1 AL2 AL3 AL4 AL1' AL2' AL3' AL4' L1 L2 L1' L2' :
-      inRel R AL1 AL2 AL3 AL4 L1 L2
-      -> mutual_block (R (AL1'++AL1) (AL2'++AL2) (AL3'++AL3) (AL4'++AL4) (L1'++L1) (L2'++L2))
-                     0 AL1' AL2' AL3' AL4' L1' L2'
-      -> inRel R (AL1'++AL1) (AL2'++AL2) (AL3'++AL3) (AL4'++AL4) (L1'++L1) (L2'++L2).
-
 Inductive approx
-  : list params
-    -> list (set var)
-    -> list (option (set var))
-    -> list params
-    -> list I.block
-    -> list I.block
-    -> params
-    -> set var
-    -> option (set var)
-    -> params
-    -> I.block
-    -> I.block -> Prop :=
+  : list params -> list (set var) -> list (option (set var)) -> list params -> list I.block -> list I.block
+    -> params -> set var -> option (set var) -> params -> I.block -> I.block -> Prop :=
   blk_approxI o (Za Z':list var) ZL Lv DL ZAL s ans ans_lv ans_lv' n L1 L2
               (RD:forall G, o = Some G ->
                        live_sound Imperative (@List.app _ ⊜ ZL ZAL) Lv (compile ZAL s ans) ans_lv'
@@ -87,257 +20,18 @@ Inductive approx
   -> length ZL = length Lv
   -> approx ZL Lv DL ZAL L1 L2 Z' (getAnn ans_lv') o Za (I.blockI Z' s n) (I.blockI (Z'++Za) (compile ZAL s ans) n).
 
-Lemma mutual_block_restrict AL1' AL1 AL2' AL2 AL3' AL3 AL4' AL4 L1' L1 L2' L2 G n
-  : mutual_block
-      (approx AL1 AL2 AL3 AL4 L1 L2) n AL1' AL2' AL3' AL4' L1' L2'
-    -> mutual_block (approx AL1 AL2 (restr G ⊝ AL3) AL4 L1 L2)
-                   n AL1' AL2' (restr G ⊝ AL3') AL4' L1' L2'.
-Proof.
-  intros. general induction H; eauto using @mutual_block.
-  simpl.
-  econstructor; eauto.
-  inv H2. econstructor; eauto with len.
-  intros.
-  destruct a3; isabsurd; simpl in *; cases in H4; isabsurd.
-  edestruct RD; eauto.
-  split; eauto. rewrite restrict_idem; eauto.
-Qed.
-
 Lemma approx_restrict ZL Lv DL ZAL L L' G
   : inRel approx ZL Lv DL ZAL L L'
     -> inRel approx ZL Lv (restr G ⊝ DL) ZAL L L'.
 Proof.
-  intros IR.
-  general induction IR; simpl in *; eauto using @inRel.
-  - rewrite List.map_app. econstructor; eauto.
-    rewrite <- List.map_app.
-    eapply mutual_block_restrict. eauto.
+  eapply inRel_map_A3.
+  intros. inv H. econstructor; eauto with len.
+  intros. destruct a3; simpl in *; isabsurd.
+  cases in H2; isabsurd.
+  exploit RD; eauto; dcr.
+  split; eauto.
+  rewrite restrict_idem; eauto.
 Qed.
-
-
-Definition defined_on {X} `{OrderedType X} {Y} (G:set X) (E:X -> option Y)
-  := forall x, x ∈ G -> exists y, E x = Some y.
-
-Lemma defined_on_update_some X `{OrderedType X} Y (G:set X) (E:X -> option Y) x v
-  : defined_on (G \ {{x}}) E
-    -> defined_on G (E [x <- Some v]).
-Proof.
-  unfold defined_on; intros. lud.
-  - eauto.
-  - eapply H0; eauto. cset_tac; intuition.
-Qed.
-
-Lemma defined_on_incl X `{OrderedType X} Y (G G':set X) (E:X -> option Y)
-  : defined_on G E
-    -> G' ⊆ G
-    -> defined_on G' E.
-Proof.
-  unfold defined_on; intros; eauto.
-Qed.
-
-Lemma omap_var_defined_on Za lv E
-: of_list Za ⊆ lv
-  -> defined_on lv E
-  -> exists l, omap (exp_eval E) (List.map Var Za) = Some l.
-Proof.
-  intros. general induction Za; simpl.
-  - eauto.
-  - simpl in *.
-    edestruct H0.
-    + instantiate (1:=a). cset_tac; intuition.
-    + rewrite H1; simpl. edestruct IHZa; eauto.
-      cset_tac; intuition.
-      rewrite H2; simpl. eauto.
-Qed.
-
-Lemma defined_on_update_list lv (E:onv val) Z vl
-: length vl = length Z
-  -> defined_on (lv \ of_list Z) E
-  -> defined_on lv (E [Z <-- List.map Some vl]).
-Proof.
-  unfold defined_on; intros.
-  decide (x ∈ of_list Z).
-  - eapply length_length_eq in H. clear H0.
-    general induction H; simpl in * |- *.
-    + exfalso. cset_tac; intuition.
-    + lud; eauto. edestruct IHlength_eq; eauto. cset_tac; intuition.
-  - edestruct H0; eauto. instantiate (1:=x). cset_tac; intuition.
-    exists x0. rewrite <- H2.
-    eapply update_with_list_no_update; eauto.
-Qed.
-
-(*
-Lemma mutual_approx_impl {A} {B} `{BlockType B} {C} `{BlockType C}
-      (R: list A -> list B -> list C -> A -> B -> C -> Prop)
-      (AL:list A) DL F1 F2 AL' F1' F2' i L1 L2
-  : length AL = length F1
-    -> length F1 = length F2
-    -> F1' = drop i F1
-    -> F2' = drop i F2
-    -> AL' = drop i AL
-    -> (forall n a b b', get AL n a -> get F1 n b -> get F2 n b' -> R DL L1 L2 a b b')
-    -> (forall i b, get F1 i b -> i = block_n b)
-    -> (forall i b, get F2 i b -> i = block_n b)
-    -> mutual_block (R DL L1 L2) i AL' F1' F2'.
-Proof.
-  intros LenEq1 LenEq2 LenF1' LenF2' LenAL' GET I1 I2.
-  assert (LenAL1:length_eq AL' F1'). subst; eauto using drop_length_stable with len.
-  assert (LenAL2:length_eq AL' F2'). subst; eauto using drop_length_stable with len.
-  general induction LenAL1; inv LenAL2; eauto using @mutual_block.
-  - econstructor; eauto using drop_eq.
-    eapply IHLenAL1; eauto using drop_shift_1.
-Qed.
- *)
-
-(*
-
-Lemma approx_mutual_block n ZL DL F F' Za Za' ans ans' ans_lv ans_lv' als als' Lv L1X L2X
-      (LEN1:length F = length Za)
-      (LEN2:length F = length ans_lv)
-      (LEN3:length F = length ans)
-      (LEN4:length F = length als)
-      (LEN5:length DL = length ZL)
-      (LEN6:length ZL = length Lv)
-      (DROP1:F' = drop n F)
-      (DROP2:Za' = drop n Za)
-      (DROP3:ans' = drop n ans)
-      (DROP4:ans_lv' = drop n ans_lv)
-      (DROP5:als' = drop n als)
-      (TRS: forall (n : nat) (ans' : ann (list params))
-              (lvs : ann (set var)) (Zs : params * stmt)
-              (Zx : params),
-          get ans_lv n lvs ->
-          get F n Zs ->
-          get Za n Zx ->
-          get ans n ans' ->
-          trs
-            (restrict (mkGlobals F Za ans_lv ++ DL)
-                      (getAnn lvs \ of_list (fst Zs ++ Zx)))
-            (Za ++ ZL) (snd Zs) lvs ans')
-      (LIVE : forall (n : nat) (Zs : params * stmt) (a : ann (set var)),
-          get (compileF compile ZL F Za Za ans) n Zs ->
-          get als n a ->
-          live_sound Imperative
-                     ( zip pair (getAnn ⊝ als) (fst ⊝ (compileF compile ZL F Za Za ans)) ++ Lv) (snd Zs) a)
-  : mutual_block
-      (approx
-         (zip pair
-              (zip pair
-                   (zip pair (getAnn ⊝ als) (fst ⊝ (compileF compile ZL F Za Za ans)))
-                   (mkGlobals F Za ans_lv)) Za ++ zip pair (zip pair Lv DL) ZL) L1X L2X)
-      n
-      (zip pair
-           (zip pair
-                (zip pair (getAnn ⊝ als') (fst ⊝ (compileF compile ZL F' Za' Za ans')))
-                (mkGlobals F' Za' ans_lv')) Za')
-      (mapi_impl I.mkBlock n F')
-      (mapi_impl I.mkBlock n (compileF compile ZL F' Za' Za ans')).
-Proof with eapply length_length_eq; subst; eauto using drop_length_stable.
-  unfold compileF.
-  assert (LEN1':length_eq F' Za'). eauto...
-  assert (LEN2':length_eq F' ans_lv'). eauto...
-  assert (LEN3':length_eq F' ans'). eauto...
-  assert (LEN4':length_eq F' als'). eauto...
-  general induction LEN1'; inv LEN2'; inv LEN3'; inv LEN4'.
-  - econstructor.
-  - simpl. econstructor; eauto.
-    + eapply IHLEN1'; eauto using drop_shift_1.
-    + unfold I.mkBlock. simpl fst. simpl snd.
-      rewrite <- zip_app.
-      rewrite <- zip_app; eauto 20 with len.
-      econstructor; eauto 20 with len.
-      intros. invc H0. split.
-      exploit LIVE; eauto 30 using zip_get, drop_eq; eauto with len.
-      exploit TRS; eauto 30 using zip_get, drop_eq; eauto with len.
-      rewrite of_list_app in H0. rewrite <- minus_union in H0. eauto.
-      repeat rewrite zip_length2; eauto 20 with len.
-Qed.
- *)
-
-Global Instance update_with_list_inst X `{OrderedType X} Y `{OrderedType Y} :
-  Proper (eq ==> (list_eq (option_eq eq)) ==> (@feq X (option Y) eq ) ==> (@feq _ _ eq))
-         (@update_with_list X _ (option Y)).
-Proof.
-  unfold respectful, Proper; intros. subst.
-  general induction H2; simpl; eauto.
-  - destruct y; simpl; eauto.
-  - destruct y; simpl; eauto.
-    hnf; intros. lud.
-    inv H; eauto.
-    eapply IHlist_eq; eauto.
-Qed.
-
-Lemma inRel_less {A1 A2 A3 A4:Type} {B} `{BlockType B} {C} `{BlockType C}
-      (R:list A1 -> list A2 -> list A3 -> list A4 -> list B -> list C ->
-         A1 -> A2 -> A3 -> A4 -> B -> C -> Prop)
-      AL1 AL2 AL3 AL4 (L:list B) (L':list C) n b
-: inRel R AL1 AL2 AL3 AL4 L L' -> get L n b -> block_n b <= n.
-Proof.
-  intros. general induction H1. inv H2; eauto.
-  eapply get_app_cases in H3; destruct H3; dcr.
-  erewrite mutual_block_zero; eauto. omega.
-  rewrite IHinRel; try eapply H4. omega.
-Qed.
-
-Lemma inRel_drop {A1 A2 A3 A4:Type} {B} `{BlockType B} {C} `{BlockType C}
-      (R:list A1 -> list A2 -> list A3 -> list A4 -> list B -> list C ->
-         A1 -> A2 -> A3 -> A4 -> B -> C -> Prop)
-      AL1 AL2 AL3 AL4 (L:list B) (L':list C) n b
-: inRel R AL1 AL2 AL3 AL4 L L'
-  -> get L n b
-  -> inRel R
-          (drop (n - block_n b) AL1)
-          (drop (n - block_n b) AL2)
-          (drop (n - block_n b) AL3)
-          (drop (n - block_n b) AL4)
-          (drop (n - block_n b) L)
-          (drop (n - block_n b) L').
-Proof.
-  intros. general induction H1; simpl; eauto; isabsurd.
-  - eapply get_app_cases in H3; destruct H3; dcr.
-    + exploit (mutual_block_zero H2 H3); eauto.
-      rewrite H4. orewrite (n - (n + 0)= 0). simpl; econstructor; eauto.
-    + exploit (inRel_less H1 H4); eauto.
-      specialize (IHinRel _ _ H4).
-      assert (length L1' + (n - length L1') = n) by omega.
-      rewrite <- H6.
-      orewrite (length L1' + (n - length L1') - block_n b
-                = length L1' + (n - length L1' - block_n b)).
-      exploit (mutual_block_length H2); dcr.
-Admitted.
-
-Lemma inRel_nth {A} {B} `{BlockType B} {C} `{BlockType C} R
-      (AL:list A) (L:list B) (L':list C) n b
-: inRel R AL L L' -> get L n b ->
-  exists a:A, exists c:C,
-    get AL n a /\ get L' n c /\ R (drop (n - block_n b) AL) (drop (n - block_n b) L) (drop (n - block_n b) L') a b c.
-Proof.
-  intros. general induction H1; isabsurd.
-  eapply get_app_cases in H3; destruct H3; dcr.
-  - exploit (mutual_block_zero H2 H3); eauto. rewrite H4.
-    orewrite (n - (n + 0) = 0). simpl.
-    edestruct (mutual_block_get H2 H3) as [? [? [? []]]].
-    do 2 eexists. repeat split; eauto using get_app.
-  - edestruct IHinRel; eauto; dcr. do 2 eexists.
-    pose proof (mutual_block_length H2); dcr.
-    repeat split; try (eapply get_app_right; eauto; omega).
-    orewrite (n = length L1' + (n - length L1')).
-    exploit (inRel_less H1 H4).
-    orewrite (length L1' + (n - length L1') - block_n b
-              = length L1' + (n - length L1' - block_n b)).
-    Typeclasses eauto :=10.
-    rewrite <- H8 at 1. repeat rewrite drop_app. rewrite H10. rewrite drop_app.
-    rewrite <- H10. eauto.
-Qed.
-
-Tactic Notation "inRel_invs" :=
-match goal with
-  | [ H : inRel ?R ?A ?B ?C, H' : get ?B ?n ?b |- _ ] =>
-    let InR := fresh "InR" in let G := fresh "G" in
-    edestruct (inRel_nth H H') as [? [? [? [G InR]]]]; (try eassumption); dcr; inversion InR; try subst;
-    let X'' := fresh "H" in pose proof (inRel_drop H H') as X'';
-    repeat get_functional; (try subst)
-end.
 
 Lemma trsR_sim (E E':onv val) L L' s ans Lv' ans_lv ans_lv' DL ZL ZAL
   (RD: trs DL ZAL s ans_lv ans)
@@ -368,55 +62,27 @@ Proof.
     + no_step.
   - no_step. simpl. rewrite EQ; eauto.
   - simpl counted in *.
-    erewrite get_nth_default; eauto.
-    erewrite get_nth_default in H8; eauto.
+    erewrite get_nth in *; eauto.
     case_eq (omap (exp_eval E) Y); intros.
-    +
-(*    exploit (@zip_get _ _ _ pair Lv' DL); eauto.
-    exploit (@zip_get _ _ _ pair (zip pair Lv' DL) ZL); eauto.
-    simpl in *.
-    inRel_invs.
-    erewrite get_nth_default in H6; eauto.
-    edestruct (omap_var_defined_on Za); eauto.
-    eapply get_in_incl; intros.
-    exploit H8. eapply get_app_right. Focus 2.
-    eapply map_get_1; eauto. reflexivity. inv H11; eauto.
-    + (*exploit get_drop_eq; try eapply LEN1; eauto. subst o.
-      exploit get_drop_eq; try eapply H11; eauto. subst x.*)
-      one_step.
-      * simpl; eauto.
-        repeat rewrite app_length in H6. rewrite map_length in H6.
-        omega.
-      * instantiate (1:=l ++ x).
-        rewrite omap_app.
-        erewrite omap_agree. Focus 2.
-        intros. rewrite <- EQ. reflexivity.
-        rewrite H10; simpl. rewrite H1; simpl. reflexivity.
-      * exploit RD0; eauto; dcr. simpl.
-        eapply trsR_sim. econstructor. eauto.
-        eapply approx_restrict.
-        Focus 3.
-        instantiate (1:=Lv).
-        erewrite H9.
-        eapply (inRel_drop EA H7).
-        congruence. congruence.
-        simpl. rewrite List.map_app.
-        rewrite update_with_list_app.
-        rewrite (omap_self_update E' Za H10). rewrite EQ. reflexivity.
-        rewrite map_length.
-        exploit omap_length; try eapply H0; eauto.
-        exploit omap_length; try eapply H1; eauto.
-        repeat rewrite app_length in H6. rewrite map_length in H6. omega.
-        eauto.
-        eapply defined_on_update_list; eauto using defined_on_incl.
-        exploit omap_length; try eapply H0; eauto.
-        exploit omap_length; try eapply H1; eauto.
-        rewrite map_length in H11.
-        repeat rewrite app_length in H6. rewrite map_length in H6.
-        repeat rewrite app_length. omega.
-        rewrite restrict_length. simpl in H7.
-        congruence. congruence.*)
-      admit.
+    + inv_get.
+      assert (❬Y❭ = ❬x❭). {
+        repeat rewrite app_length in H8.
+        rewrite map_length in H8. omega.
+      }
+      inRel_invs. inv H12; simpl in *.
+      edestruct (omap_var_defined_on Za); eauto.
+      eapply get_in_incl. intros.
+      exploit H10; eauto using get_app_right. inv H14; eauto.
+      one_step. rewrite omap_app.
+      erewrite omap_agree with (g:=exp_eval E). rewrite H1.
+      simpl. rewrite H9. reflexivity. intros. rewrite EQ; eauto.
+      simpl. exploit RD0; eauto; dcr.
+      eapply trsR_sim; eauto using approx_restrict with len.
+      * rewrite EQ. rewrite List.map_app.
+        rewrite update_with_list_app; eauto with len.
+        rewrite (omap_self_update _ _ H9); reflexivity.
+      * eapply defined_on_update_list; eauto with len.
+        eapply defined_on_incl; eauto.
     + no_step.
       rewrite omap_app in def. monad_inv def.
       erewrite omap_agree in H1. erewrite H1 in EQ0. congruence.
