Alpha.v
@@ -353,8 +353,7 @@ Proof.
       erewrite omap_agree_2; eauto. intros. symmetry.
       eapply alpha_exp_eval. eapply H0; eauto; eauto. hnf; intros; eauto.
       simpl. eapply alphaSim_sim; econstructor; eauto using PIR2_drop.
-      eapply envCorr_update_list; eauto. exploit omap_length; eauto.
-      rewrite map_length. congruence.
+      eapply envCorr_update_list; eauto with len.
     + no_step. erewrite omap_agree_2 in H1; try eapply H.
       erewrite H1 in def. congruence.
       intros. eapply alpha_exp_eval. eapply H0; eauto. eauto.
