Coherence/AllocationValidator.v
@@ -11,45 +11,54 @@ Definition srd_dec DL s a
 Proof.
   hnf. revert DL a.
   sinduction s; simpl.
-  + edestruct a as [|lv a'| |]; try dec_solve.
-    edestruct (X x0); try dec_solve; eauto.
-  + edestruct a as [?|?|lv als alt|]; try dec_solve.
-    edestruct (X x1), (X x2); try dec_solve; eauto.
-  + destruct a;
-    destruct (get_dec DL (counted l)) as [[[G'|] ?]|?];
-    try dec_solve.
-  + destruct a; try dec_solve.
-  + edestruct a as [|lv a'| |]; try dec_solve.
-    edestruct (X x0); try dec_solve; eauto.
-  + destruct a as [?|?|lv als alt| ]; try dec_solve.
-    decide (length s = length sa); try dec_solve.
-    edestruct (X x) with (DL:=oglobals s sa++DL); eauto; try dec_solve.
+  + edestruct a as [|lv a'| |]; [dec_right| | dec_right| dec_right].
+    edestruct (X x0); [ eauto | dec_solve | dec_right].
+  + edestruct a as [?|?|lv als alt|]; [dec_right| dec_right| | dec_right].
+    edestruct (X x1), (X x2); eauto; [ | dec_right| |dec_right ]; dec_solve.
+  + destruct a; [ | dec_right | dec_right | dec_right].
+    destruct (get_dec DL (counted l)) as [[[G'|] ?]|?]; [| dec_right | dec_right].
+    dec_solve.
+  + destruct a; [ | dec_right | dec_right | dec_right]. dec_solve.
+  + edestruct a as [|lv a'| |]; [dec_right| | dec_right| dec_right].
+    edestruct (X x0); eauto; [| dec_right]. dec_solve; eauto.
+  + destruct a as [?|?|lv als alt| ]; [dec_right| dec_right| dec_right|].
+    ensure (length s = length sa).
+    edestruct (X x) with (DL:=Some ⊝ (getAnn ⊝ sa) \\ (fst ⊝ s) ++ DL); eauto; [ |dec_right].
     edestruct (indexwise_R_dec'
-                 (R:=fun x y => srd (restrict (oglobals s sa ++ DL) (getAnn y \ of_list (fst x))) (snd x) y) (LA:=s) (LB:=sa));
-      try dec_solve.
+                 (R:=fun x y =>
+                       srd (restr (getAnn y \ of_list (fst x))
+                                  ⊝ (Some ⊝ (getAnn ⊝ sa) \\ (fst ⊝ s) ++ DL))
+                           (snd x) y) (LA:=s) (LB:=sa)).
     intros. eapply X; eauto.
+    dec_solve. dec_right.
     Grab Existential Variables. eauto. eauto. eauto. eauto.
 Defined.
 
 (** ** local injectivity is decidable *)
 
+
+Local Hint Extern 1 =>
+match goal with
+  [ H : annotation _ _ |- annotation _ _ ] => inv H; eassumption
+end.
+
 Definition locally_inj_dec (ϱ:env var) (s:stmt) (lv:ann (set var)) (an:annotation s lv)
   : {locally_inj ϱ s lv} + {~ locally_inj ϱ s lv}.
 Proof.
   revert ϱ lv an.
-  sind s; intros; destruct s; destruct lv; try (now exfalso; inv an).
-  + decide(injective_on a ϱ); try dec_solve.
-    edestruct (IH s); eauto; try dec_solve. inv an; eauto.
-  + decide(injective_on a ϱ); try dec_solve;
-    edestruct (IH s1); eauto; try inv an; eauto; try dec_solve;
-    edestruct (IH s2); eauto; try inv an; eauto; try dec_solve.
-  + decide(injective_on a ϱ); try dec_solve.
-  + decide(injective_on a ϱ); try dec_solve.
-  + decide(injective_on a ϱ); try dec_solve;
-    edestruct (IH s); eauto; try dec_solve; inv an; eauto.
-  + decide(injective_on a ϱ); try dec_solve.
-    decide(length s = length sa); try dec_solve.
-    edestruct (IH s0); eauto; try inv an; eauto; try dec_solve.
+  sind s; intros; destruct s; destruct lv; try solve [ exfalso; inv an ].
+  + ensure (injective_on a ϱ).
+    edestruct (IH s); eauto. dec_solve. dec_right.
+  + ensure (injective_on a ϱ).
+    edestruct (IH s1); eauto; [|dec_right].
+    edestruct (IH s2); eauto; [|dec_right]. dec_solve.
+  + ensure (injective_on a ϱ); dec_solve.
+  + ensure (injective_on a ϱ); dec_solve.
+  + ensure (injective_on a ϱ).
+    edestruct (IH s); eauto; [| dec_right]. dec_solve.
+  + ensure (injective_on a ϱ).
+    ensure (length s = length sa).
+    edestruct (IH s0); eauto; [| dec_solve].
     edestruct (indexwise_R_dec' (R:=fun x y => locally_inj ϱ (snd x) y) (LA:=s) (LB:=sa));
       try dec_solve.
     intros. eapply IH; eauto. inv an; eauto.
