Coherence/Coherence.v
@@ -178,23 +178,6 @@ Qed.
 
 (** *** In a coherent program, the globals of every function that can eventually be called are live *)
 
-Lemma restrict_ifFstR B (R:⦃var⦄->B->Prop) DL GL G
-: PIR2 (ifFstR R) DL GL
-  -> PIR2 (ifFstR R) (restr G ⊝ DL) GL.
-Proof.
-  intros. induction H; simpl; eauto using PIR2, @ifFstR.
-  unfold restr. destruct pf.
-  - eauto using @PIR2, @ifFstR.
-  - cases; eauto using PIR2, @ifFstR.
-Qed.
-
-Lemma PIR2_ifFstR_refl A (R:A->A->Prop) `{Reflexive _ R} L
-  : PIR2 (ifFstR R) (Some ⊝ L) L.
-Proof.
-  eapply PIR2_get; intros; inv_get; eauto using @ifFstR with len.
-Qed.
-
-
 Lemma srd_globals_live s ZL Lv DL alv f
 : live_sound Imperative ZL Lv s alv
   -> srd DL s alv
