Coherence/DelocationValidator.v
@@ -4,46 +4,53 @@ Require Import Liveness Restrict Delocation Indexwise.
 Set Implicit Arguments.
 Unset Printing Records.
 
+Local Hint Extern 1 =>
+match goal with
+  [ H : annotation _ _ |- annotation _ _ ] => inv H; eassumption
+end.
+
 Lemma trs_dec DL ZL s ans_lv ans
   : {trs DL ZL s ans_lv ans} +
     {~ trs DL ZL s ans_lv ans}.
 Proof.
   revert DL ZL ans_lv ans.
-  sind s. destruct s; destruct ans; try dec_solve;
-  destruct ans_lv; try dec_solve.
-  + destruct a; edestruct (IH s (ltac:(eauto)) (restrict DL (a0\ singleton x)) ZL ans_lv ans);
-    try dec_solve.
-  + destruct a; subst; try dec_solve;
-    destruct (IH s1 (ltac:(eauto)) DL ZL ans_lv1 ans1); try dec_solve;
-    destruct (IH s2 (ltac:(eauto)) DL ZL ans_lv2 ans2); try dec_solve.
-  + destruct (get_dec DL (counted l)) as [[[G'|]]|];
-    destruct (get_dec ZL (counted l)) as [[Za ?]|];
-    try destruct a;
-    try decide (G' ⊆ a0);
-    try decide (of_list (Za) ⊆ a0);
-    subst; try dec_solve; try inv an; try inv an_lv; eauto.
-  + decide (a = nil);
-    subst; try dec_solve; try inv an; try inv an_lv; eauto.
-  + destruct a; edestruct (IH s (ltac:(eauto)) (restrict DL (a0\ singleton x)) ZL ans_lv ans); try dec_solve.
-  + decide (length s = length a);
-    decide (length s = length sa);
-    decide (length s = length sa0); try dec_solve.
-    destruct (IH s0 (ltac:(eauto)) (mkGlobals s a sa0 ++ DL) (a ++ ZL) ans_lv ans); try dec_solve.
+  sind s.
+  time (destruct s; destruct ans; try solve [dec_right]; destruct ans_lv; try solve [dec_right]).
+  + destruct a; [ | dec_right];
+      destruct (IH s (ltac:(eauto)) (restr (a0\ singleton x) ⊝  DL) ZL ans_lv ans); [| dec_right].
+    dec_solve.
+  + destruct a; [| dec_right];
+    destruct (IH s1 (ltac:(eauto)) DL ZL ans_lv1 ans1); [| dec_right];
+    destruct (IH s2 (ltac:(eauto)) DL ZL ans_lv2 ans2); [| dec_right].
+    dec_solve.
+  + destruct (get_dec DL (counted l)) as [[[G'|]]|];[| dec_right | dec_right];
+    destruct (get_dec ZL (counted l)) as [[Za ?]|]; [| dec_right];
+      destruct a; [| dec_right];
+        dec_solve.
+  + destruct a;[| dec_right].
+    dec_solve.
+  + destruct a;[| dec_right].
+    edestruct (IH s (ltac:(eauto)) (restr (a0\ singleton x) ⊝ DL) ZL ans_lv ans); try dec_solve.
+  + ensure (length s = length a);
+    ensure (length s = length sa);
+    ensure(length s = length sa0).
+    destruct (IH s0 (ltac:(eauto)) (Some ⊝ (getAnn ⊝ sa0) \\ app (A:=var) ⊜ (fst ⊝ s) a ++ DL)
+                 (a ++ ZL) ans_lv ans);[| dec_right].
     edestruct (indexwise_R4_dec
-                 (R:=fun lvs Zs Za' ans' => trs (restrict (mkGlobals s a sa0 ++ DL)
-                                                         (getAnn lvs \ of_list (fst Zs ++ Za')))
-                                               (a ++ ZL) (snd Zs) lvs ans')
+                 (R:=fun lvs Zs Za' ans' =>
+                       trs (restr (getAnn lvs \ of_list (fst Zs ++ Za'))
+                                     ⊝ (Some ⊝ (getAnn ⊝ sa0) \\ app (A:=var) ⊜ (fst ⊝ s) a ++ DL))
+                           (a ++ ZL) (snd Zs) lvs ans')
                  (LA:=sa0)
                  (LB:=s)
                  (LC:=a)
                  (LD:=sa)); intros; eauto.
     hnf; intros. eapply IH; eauto.
-    dec_solve. dec_solve.
+    dec_solve. dec_right.
 Defined.
 
 Instance trs_dec_inst DL ZL s lv Y
 : Computable (trs DL ZL s lv Y).
 Proof.
-  try (now right; intro A; eapply trs_annotation in A; dcr; eauto).
   hnf; eauto using trs_dec.
 Defined.
