Constr/MapDefined.v
@@ -1,0 +1,43 @@
+Require Export Setoid Coq.Classes.Morphisms.
+Require Import EqDec Computable Util AutoIndTac.
+Require Export CSet  Containers.SetDecide.
+Require Export MapBasics MapLookup MapUpdate.
+
+Set Implicit Arguments.
+
+Definition defined_on {X} `{OrderedType X} {Y} (G:set X) (E:X -> option Y)
+  := forall x, x ∈ G -> exists y, E x = Some y.
+
+Lemma defined_on_update_some X `{OrderedType X} Y (G:set X) (E:X -> option Y) x v
+  : defined_on (G \ {{x}}) E
+    -> defined_on G (E [x <- Some v]).
+Proof.
+  unfold defined_on; intros. lud.
+  - eauto.
+  - eapply H0; eauto. cset_tac; intuition.
+Qed.
+
+Lemma defined_on_incl X `{OrderedType X} Y (G G':set X) (E:X -> option Y)
+  : defined_on G E
+    -> G' ⊆ G
+    -> defined_on G' E.
+Proof.
+  unfold defined_on; intros; eauto.
+Qed.
+
+Lemma defined_on_update_list X `{OrderedType X} Y lv (E: X -> option Y) Z vl
+: length vl = length Z
+  -> defined_on (lv \ of_list Z) E
+  -> defined_on lv (E [Z <-- List.map Some vl]).
+Proof.
+  unfold defined_on; intros.
+  decide (x ∈ of_list Z).
+  - length_equify. clear H1.
+    general induction H0; simpl in * |- *.
+    + exfalso. cset_tac.
+    + lud; eauto.
+      eapply IHlength_eq; eauto; cset_tac; intuition.
+  - edestruct H1; eauto. cset_tac.
+    exists x0. rewrite <- H3.
+    eapply update_with_list_no_update; eauto.
+Qed.
