Infra/DecSolve.v
@@ -1,6 +1,12 @@
 Require Import Util Computable Get.
 
 
-Ltac dec_solve := solve [ left; econstructor; eauto 
+Ltac dec_solve := solve [ left; econstructor; eauto
                         | let H := fresh "H" in right; intro H; inv H; repeat get_functional; isabsurd; eauto ].
 
+
+Tactic Notation "dec_right" :=
+  let A := fresh "A" in
+  right; intro A; inv A; repeat get_functional; eauto.
+
+Tactic Notation "ensure" constr(P) := decide P; [ | dec_right].
